\documentclass[12pt,twoside]{article}
\usepackage[dvipsnames]{xcolor}
\usepackage{tikz,graphicx,amsmath,amsfonts,amscd,amssymb,bm,cite,epsfig,epsf,url}
\usepackage[hang,flushmargin]{footmisc}
\usepackage[colorlinks=true,urlcolor=blue,citecolor=blue]{hyperref}
\usepackage{amsthm,multirow,wasysym,appendix}
\usepackage{array,subcaption} 
% \usepackage[small,bf]{caption}
\usepackage{bbm}
\usepackage{pgfplots}
\usetikzlibrary{spy}
\usepgfplotslibrary{external}
\usepgfplotslibrary{fillbetween}
\usetikzlibrary{arrows,automata}
\usepackage{thmtools}
\usepackage{blkarray} 
\usepackage{textcomp}
\usepackage{pgf,tikz}
\usepackage{pgfplots}
\usepackage[left=0.8in,right=1.0in,top=1.0in,bottom=1.0in]{geometry}

\input{macros}

\begin{document}

\begin{center}
{\large{\textbf{Homework 0}} } \vspace{0.2cm}\\
Due September 12 at 11 pm
\\
\end{center}
Name: Giulio Duregon

\begin{enumerate}

\item (Sets) We will use set theory to define probability spaces. Are these statements true or false? Provide a proof if they are true (you can use Venn diagrams to gain intuition, but also write down a formal proof), or a counterexample if they are false. 
\begin{enumerate}
\item[] A partition of a set $\Omega$ is a collection of sets $S_1$, \ldots, $S_n$ such that $\Omega = \cup_{i}S_i$ and $S_i \cap S_j = \emptyset$ for $i\neq j$. 
\item If  $S_1$, \ldots, $S_n$ is a partition of $\Omega$, then for any subset $A \subseteq \Omega$, $S_1 \cap A$, \ldots, $S_n \cap A$ is a partition of $A$.
\subitem
This statement is true, as $A = \cup_{i}S_i \cap A$ (I'm not sure if I wrote this correctly mathematically, but what I'm trying to say is that if we add (by taking the union) all the intersections between $A$ and $S_1, \dots, S_n$ they will add up to A).\par
Also,  $(A \cap S_i) \cap (A \cap S_j) = \emptyset$ for $i\neq j$ (Again, not sure if I wrote this correctly, but what I am trying to express is that since $S_1, \dots, S_n$ is a partition of $\Omega$ by definition it is disjoint, so every $A\cap S_i$ will be disjoint from every other $A\cap S_j$ where $i\neq j$).

\item For any sets $A$ and $B$, $A^c \cup B^c = (A \cup B)^c$. 
\subitem This statement is false, which will be proven by counter example. Consider the sample space where $A,B \in \Omega$ and $A \cap B \neq \emptyset$ (I am trying to describe the classic ven-diagram where A and B exist in a sample space and share some area). In this case the statement $A^c \cup B^c$ is the area outside of the ven diagrams. The statement $(A \cup B)^c$ however, contains all the area of the sample space except for $A \cap B$. Therefore, the two areas are not equal. See picture at the end of pdf for illustration. 
\item For any sets $A$, $B$, and $C$, $(A \cup B) \cap C = A \cup (B \cap C)$. 
\subitem
This is false by counter example. Consider the sample space $\Omega$ where $A,B,C \in \Omega$ and $A\cap B, A\cap C, B\cap C$ and $A\cap B \cap C \neq \emptyset$. (Here I am trying to illustrate a sample space with the triple ven diagram, where A,B,C have overlap). The statement  $(A \cup B) \cap C$ contains the areas $A\cap B, A \cap C, A\cap B \cap C$. The statement $ A \cup (B \cap C)$ however, contains the areas $A, A\cap B, A\cap C, A\cap B \cap C$ Therefore what our statement of says is: 
\begin{equation}
    \begin{split}
        A\cap B + A\cap C + A\cap B \cap C = A + B \cap C
    \end{split}
\end{equation}
Which we can clearly see is not true. See picture at the end of pdf for illustration.
\end{enumerate}
% \vspace{0.4cm}

\break
\item (Series) We will need series to compute probabilities and expectations related to discrete quantities. 
 \begin{enumerate}
\item  Assuming $r\neq 1$, derive a simple expression for
\begin{align}
S_n := \sum_{i=m}^{n} r^{i}
\end{align}
as a function of $r$, $m$ and $n$, and prove that it holds. Assume $m$
and $n$ are positive integers with $m\leq n$.
\subitem
To solve this geometric series we're going to do the following 5 steps: \\
1) Unwrap the series into a form we can perform algebraic manipulations on     \\
2) Multiply both sides by r \\
3) Subtract our $S_n$ statement by our $rS_n$ statement\\
4) Factor out $(1-r)$ from both sides \\
5) Isolate $S_n$ and we have our answer


\begin{equation} \label{eq1}
\begin{split}
S_n := r^m + r^{m+1} + \dots + r^n \\ 
r\times S_n := r\times r^m + r\times r^{m+1} + \dots + r\times r^n \\
S_n - r\times S_n := r - r\times r^n \\
S_n(1-r) = r(1-r^n) \\ 
Sn = \frac{r(1-r^n)}{1-r}
\end{split}
\end{equation}

\item Under what condition on $r$ does the infinite series
\begin{align}
\sum_{i=m}^{\infty} r^{i} = \lim_{n \rightarrow \infty} S_n
\end{align}
converge (where again $m$ is a positive integer)?  
\subitem
The series converges at $k$ where $-1<k<1$ holds true. If $k=1$ the series is undefined (division by 0), and if $k=-1$ Otherwise the series expands to $\pm \infty$ and never converges.
\item Use induction to prove the identity
\begin{align}
\sum_{i=1}^{n} i = \frac{n(n+1)}{2},
\end{align}
where $n$ is a nonnegative integer greater than 1.
\subitem
Lets take a base case with $n=2$. We have: $(2(2+1))/2=3$ which if we check $1+2=3$ holds true.
Now assume the expression holds for $n$ where $n=k$. We would have the following:
\begin{align}
\sum_{i=1}^{k} i = \frac{k(k+1)}{2},
\end{align}
when $n = k+1$
\begin{equation}
    \begin{split}
    \sum_{i=1}^{k+1} i = \frac{(k+1)(k+1+1)}{2} =  \sum_{i=1}^{k} i +(k+1) \\
    \sum_{i=1}^{k+1} i = \frac{k(k+1)}{2} + (k+1) = \frac{(k+1)(k+2)}{2} \\
    = \frac{(k+1)(k+1+1)}{2}
    \end{split}
\end{equation}
\end{enumerate}
We've shown that the sequence holds for $n = 1$,  $n = k$, and $n=k+1$ therefore it holds for all positive integers greater than 1.

\break

\item (Derivatives)
  \begin{enumerate}
  \item Briefly explain why the derivative of a function can be interpreted as an \emph{instantaneous rate of change}.
  \subitem Answer to 3a): Derivatives calculate the slope of a tangent line between two points of a function, f(x) and f(x+h). Using the definition of the derivative, as h approaches 0, the distance between x and x+h on the x-axis becomes increasingly small, and the tangent line becomes an increasingly accurate estimate of slope. When h becomes minute, the tangent line essentially measures a rate of change a specific point, which can be interpreted as an instantaneous rate of change at that point.
  \item Use the definition to derive the derivative of the function $x^2$.
  \subitem Answer to part 3b) Use the definition of a derivative given to us, where $f(x)=x^2$. Once we get to $2x+h$, we can drop h as $h\rightarrow 0$.
  \begin{align}
    f'(x)= \lim_{h \rightarrow 0} \frac{(x+h)^2 - (x)^2}{h} \Longrightarrow \frac{(x^2+2xh+h^2)-(x^2)}{h} \Longrightarrow 
    \\ \frac{x^2}{h} - \frac{x^2}{h}+ \frac{2xh}{h} + \frac{h^2}{h} \Longrightarrow 2x+h \Longrightarrow 2x
    \end{align}
  \item We would like to approximate a differentiable function $f$ at
    $y$ using a linear function $L_y(x):=ax + b$. We set $a$ and $b$
    so that $f$ and $L_y$ have the same value and the same derivative
    at $y$ (i.e., $L_y(y)=f(y)$ and $L_y'(y)=f'(y)$). Give an
    expression for $L_{y}(x)$ in terms of $y$, $f(y)$, and $f'(y)$.  
\subitem
Start with $L_y(x):=ax + b$. We know $a$ represents the slope at the given point, so we will replace that with the derivative at that point.
$a=f'(y)$\\
Let us remember, we are using the point $y$ to approximate a point $x$. We will need to account for this by scaling our $ax$ term with the following:  $x-y$ and therefore $L_y(x):= f'(y)(x-y) + b$. \\
Lastly, $b$ is our starting point, in this case, $f(y)$\\
Thus we have $L_y(x):=f'(y)(x-y) + f(y)$
  \item Let $f(x) = 4x^2 e^{x}$. Plot $f$ and $L_{2}$ between 1 and 3. 
  \subitem
  Using the formula derived in the previous step, $f'(y)$ will be set to $f'(x) = 4x(x+2)e^x$ and $f'(2) = 32e^X$ and $b =f(2) = 16e^x $. All together we have $L_y(x) = 32e^2 \times (x-2) + 16e^2$ which we will then plot along with $f$ from the range $x=1-3$.\textbf{ The graph of the functions can be found on the last page of this pdf.}
  \end{enumerate}
  
  \break
  
 \item (Integrals) 
 \begin{enumerate}
 \item Express the area of the following shape in terms of an integral
   and solve it.
 \begin{center}
\begin{tikzpicture}
\begin{axis}[grid=major, xtick={-1,-0.75,...,1}, ytick={-1,-0.75,...,1}, xmin= -1, xmax=1, ymin=-1, ymax=1,tick label style={font=\footnotesize}]
\addplot[ very thick,samples=500] {(x-1)^2} ;
\addplot[ very thick,samples=500] {(-x-1)^2} ;
\addplot[ very thick,samples=500] {-(x-1)^2} ;
\addplot[ very thick,samples=500] {-(-x-1)^2} ;
\end{axis}
\end{tikzpicture}
\end{center}
\par
We can use the three points $(0,1), (1,0),(\frac{1}{2},\frac{1}{4})$ to determine the equation of the quadratic function in the top right corner.
The equation is $y = x^2-2x+1$, which if we integrate, we get $\frac{x^3}{3}-x^2+x+C$ and when evaluated from 0 to 1, we get $\frac{1}{3}$ as the area under the curve. However, since this is only the top right quadrant, we can leverage the x,y symmetry of the graph and multiply by 4 to find the total area. Thus the total area of the shape is $\frac{4}{3}$
  \item Use change of variables to derive a closed-form expression for the function
 \begin{align}
f(t) := \int_{0}^{t} \frac{x}{1+x^2} \diff{x}.
 \end{align}
\end{enumerate}
\subitem
So to solve this we're going to use u-substitution. Let $u= (1+x^2)$ and take the derivative of each side:
\begin{equation}
\begin{split}
   u = 1+x^2 \\
   du = 2xdx
\end{split}
\end{equation}

To solve the equation, start by substituting $u$ in for $1+x^2$, then substitute $\frac{\diff(u)}{2}$ for $x\diff{x}$, then integrate and sub $(1+x^2)$ for $u$
\begin{equation} \begin{split}
    f(t) := \int_{0}^{t} \frac{x}{u} \diff{x} \\
    \int_{0}^{t} \frac{1}{2} \frac{1}{u} \diff{u} \\
    \frac{\ln(u)}{2} + c \\
    \frac{\ln(1+x^2)}{2}+c
\end{split}
\end{equation}

  
\end{enumerate}
\break
\includegraphics{hw01b.png} 
\includegraphics{hw01c.png} \\
\includegraphics{hw03d.png}
\end{document}
